NativeLib.bpl
@@ -3,212 +3,211 @@
 // ---------------------------------------------------------------
   
 
-procedure NTransientLink#setRule(stk: Seq BoxType) returns (newStk: Seq BoxType);
-  requires Seq#Length(stk) >= 2;
-  requires typeof($Unbox(Seq#Index(stk, Seq#Length(stk)-2)):ref) == Native$TransientLink;
-  modifies Heap;
+var $srcHeap : HeapType where $IsGoodHeap($srcHeap);
+var $tarHeap : HeapType where $IsGoodHeap($tarHeap);
+var $linkHeap : HeapType where $IsGoodHeap($tarHeap);
+
+
+
+function getTarsBySrcs(Seq ref): ref;
+
+function getTarsBySrcs_inverse(ref): Seq ref;
+axiom (forall i: Seq ref :: { getTarsBySrcs(i) } getTarsBySrcs_inverse(getTarsBySrcs(i)) == i);
+
+function surj_tar_model($s: HeapType, $t: HeapType): bool
+{
+(
+forall $o: ref :: $o!=null && read($t, $o, alloc) && dtype($o) == REL$RELSchema ==>
+	(exists $i: ref :: dtype($i) == ER$ERSchema && $i != null && read($s, $i, alloc) && getTarsBySrcs(Seq#Singleton($i))==$o)
+)
+}
+
+
+procedure NTransientLink#setRule
+	(stk: Seq BoxType, link: ref, ruleName: String) 
+returns 
+	(newStk: Seq BoxType)
+  requires Seq#Length(stk) >= 2; 
+  requires $Unbox(Seq#Index(stk, Seq#Length(stk)-1)):String == ruleName;
+  requires dtype(link) == Native$TransientLink;
+  modifies $linkHeap;
+  ensures read($linkHeap, link, TransientLink#rule) == ruleName;
+  ensures (forall<T> $f: Field T :: $f!=TransientLink#rule ==> 
+	read($linkHeap, link, $f) == read(old($linkHeap), link, $f)
+  );
+  ensures (forall<alpha> $o: ref, $f: Field alpha :: { read($linkHeap, $o, $f) } $o != null && read(old($linkHeap), $o, alloc) ==> read($linkHeap, $o, $f) == read(old($linkHeap), $o, $f) || $o == link);
+  ensures $HeapSucc(old($linkHeap), $linkHeap); 
   ensures newStk == Seq#Take(stk, Seq#Length(stk)-2);
-  ensures Heap[$Unbox(Seq#Index(stk, Seq#Length(stk)-2)):ref, TransientLink#rule] == $Unbox(Seq#Index(stk, Seq#Length(stk)-1)):String;
-  ensures (forall<alpha> o:ref, f:Field alpha :: 
-	Heap[o,f] == old(Heap[o,f]) ||
-	(typeof(o)==Native$TransientLink && o == $Unbox(Seq#Index(stk, Seq#Length(stk)-2)) && f==TransientLink#rule)
-  );
- 
-
-procedure NTransientLink#addSourceElement(stk: Seq BoxType) returns (newStk: Seq BoxType);
-  requires Seq#Length(stk) >= 3;
-  requires typeof($Unbox(Seq#Index(stk, Seq#Length(stk)-3)):ref) == Native$TransientLink;
-  modifies Heap;
-  ensures newStk == Seq#Take(stk, Seq#Length(stk)-3);
-  ensures Map#Domain(Heap[$Unbox(Seq#Index(stk, Seq#Length(stk)-3)), TransientLink#source])[$Unbox(Seq#Index(stk, Seq#Length(stk)-2)): String];
-  ensures Map#Elements(Heap[$Unbox(Seq#Index(stk, Seq#Length(stk)-3)), TransientLink#source])[$Unbox(Seq#Index(stk, Seq#Length(stk)-2)): String] == $Unbox(Seq#Index(stk, Seq#Length(stk)-1));
-  ensures (forall<alpha> o:ref, f:Field alpha :: 
-	Heap[o,f] == old(Heap[o,f]) ||
-	(typeof(o)==Native$TransientLink && o == $Unbox(Seq#Index(stk, Seq#Length(stk)-3)) && f==TransientLink#source)
-  );
-  ensures (forall n: String :: n!=$Unbox(Seq#Index(stk, Seq#Length(stk)-2)): String ==>
-	Map#Domain(Heap[$Unbox(Seq#Index(stk, Seq#Length(stk)-3)), TransientLink#source])[n] == 
-	old(Map#Domain(Heap[$Unbox(Seq#Index(stk, Seq#Length(stk)-3)), TransientLink#source]))[n]
-  );	
-  ensures (forall n: String :: n!=$Unbox(Seq#Index(stk, Seq#Length(stk)-2)): String ==>
-	Map#Elements(Heap[$Unbox(Seq#Index(stk, Seq#Length(stk)-3)), TransientLink#source])[n] == 
-	old(Map#Elements(Heap[$Unbox(Seq#Index(stk, Seq#Length(stk)-3)), TransientLink#source]))[n]
-  );
- 
-procedure NTransientLink#addTargetElement(stk: Seq BoxType) returns (newStk: Seq BoxType);
-  requires Seq#Length(stk) >= 3;
-  requires typeof($Unbox(Seq#Index(stk, Seq#Length(stk)-3)):ref) == Native$TransientLink;
-  modifies Heap;
-  ensures typeof(Map#Elements(Heap[$Unbox(Seq#Index(stk, Seq#Length(stk)-3)):ref, TransientLink#target])[$Unbox(Seq#Index(stk, Seq#Length(stk)-2)):String]) == typeof($Unbox(Seq#Index(stk, Seq#Length(stk)-1)):ref);
-  ensures newStk == Seq#Take(stk, Seq#Length(stk)-3);
-  ensures Map#Domain(Heap[$Unbox(Seq#Index(stk, Seq#Length(stk)-3)), TransientLink#target])[$Unbox(Seq#Index(stk, Seq#Length(stk)-2)):String];
-  ensures Map#Elements(Heap[$Unbox(Seq#Index(stk, Seq#Length(stk)-3)), TransientLink#target])[$Unbox(Seq#Index(stk, Seq#Length(stk)-2)):String] == $Unbox(Seq#Index(stk, Seq#Length(stk)-1));
-  ensures (forall<alpha> o:ref, f:Field alpha :: 
-	Heap[o,f] == old(Heap[o,f]) ||
-	(typeof(o)==Native$TransientLink && o == $Unbox(Seq#Index(stk, Seq#Length(stk)-3)) && f==TransientLink#target)
-  );
+{
+	$linkHeap := update($linkHeap, link, TransientLink#rule, ruleName);
+	assume $IsGoodHeap($linkHeap);
+	newStk := Seq#Take(stk, Seq#Length(stk)-2);
+}
   
-procedure NTransientLink#getSourceElement(stk: Seq BoxType) returns (newStk: Seq BoxType);
-  requires typeof( $Unbox(Seq#Index(stk,Seq#Length(stk)-2)): ref ) == Native$TransientLink;
-  requires Map#Domain(Heap[$Unbox(Seq#Index(stk,Seq#Length(stk)-2)): ref, TransientLink#source])[$Unbox(Seq#Index(stk,Seq#Length(stk)-1)): String];
-  ensures newStk == Seq#Build(Seq#Take(stk, Seq#Length(stk)-2), $Box(Map#Elements(Heap[$Unbox(Seq#Index(stk,Seq#Length(stk)-2)): ref, TransientLink#source])[$Unbox(Seq#Index(stk,Seq#Length(stk)-1)): String]));
 
- 
-procedure NTransientLink#getTargetElement(stk: Seq BoxType) returns (newStk: Seq BoxType);
-  requires typeof( $Unbox(Seq#Index(stk,Seq#Length(stk)-2)): ref ) == Native$TransientLink;
-  requires Map#Domain(Heap[$Unbox(Seq#Index(stk,Seq#Length(stk)-2)): ref, TransientLink#target])[$Unbox(Seq#Index(stk,Seq#Length(stk)-1)): String];
-  ensures newStk == Seq#Build(Seq#Take(stk, Seq#Length(stk)-2), $Box(Map#Elements(Heap[$Unbox(Seq#Index(stk,Seq#Length(stk)-2)): ref, TransientLink#target])[$Unbox(Seq#Index(stk,Seq#Length(stk)-1)): String]));
+procedure  NTransientLink#addSourceElement
+	(stk: Seq BoxType, link: ref, key: String, val: ref) 
+returns 
+	(newStk: Seq BoxType)
+  requires Seq#Length(stk) >= 3; 
+  requires $Unbox(Seq#Index(stk, Seq#Length(stk)-1)):ref == val;
+  requires $Unbox(Seq#Index(stk, Seq#Length(stk)-2)):String == key;
+  requires $Unbox(Seq#Index(stk, Seq#Length(stk)-3)):ref == link;
+  requires dtype(link) == Native$TransientLink;
+  modifies $linkHeap;
+  ensures read($linkHeap, link, TransientLink#source) == Map#Build(old($linkHeap[link, TransientLink#source]), key, val);
+  ensures (forall<T> $f: Field T :: $f!=TransientLink#source ==> 
+	read($linkHeap, link, $f) == read(old($linkHeap), link, $f)
+  );
+  ensures (forall<alpha> $o: ref, $f: Field alpha :: { read($linkHeap, $o, $f) } $o != null && read(old($linkHeap), $o, alloc) ==> read($linkHeap, $o, $f) == read(old($linkHeap), $o, $f) || $o == link);
+  ensures $HeapSucc(old($linkHeap), $linkHeap); 
+  ensures newStk == Seq#Take(stk, Seq#Length(stk)-3);  
+{
+	$linkHeap := update($linkHeap, link, TransientLink#source, Map#Build($linkHeap[link, TransientLink#source], key, val));
+	assume $IsGoodHeap($linkHeap);
+	newStk := Seq#Take(stk, Seq#Length(stk)-3);
+}
   
+  
+procedure NTransientLink#addTargetElement
+	(stk: Seq BoxType, link: ref, key: String, val: ref) 
+returns 
+	(newStk: Seq BoxType)
+  requires Seq#Length(stk) >= 3; 
+  requires $Unbox(Seq#Index(stk, Seq#Length(stk)-1)):ref == val;
+  requires $Unbox(Seq#Index(stk, Seq#Length(stk)-2)):String == key;
+  requires $Unbox(Seq#Index(stk, Seq#Length(stk)-3)):ref == link;
+  requires dtype(link) == Native$TransientLink;
+  modifies $linkHeap;
+  ensures read($linkHeap, link, TransientLink#target) == Map#Build(old($linkHeap[link, TransientLink#target]), key, val);
+  ensures (forall<T> $f: Field T :: $f!=TransientLink#target ==> 
+	read($linkHeap, link, $f) == read(old($linkHeap), link, $f)
+  );
+  ensures (forall<alpha> $o: ref, $f: Field alpha :: { read($linkHeap, $o, $f) } $o != null && read(old($linkHeap), $o, alloc) ==> read($linkHeap, $o, $f) == read(old($linkHeap), $o, $f) || $o == link);
+  ensures $HeapSucc(old($linkHeap), $linkHeap); 
+  ensures newStk == Seq#Take(stk, Seq#Length(stk)-3);
+{
+	$linkHeap := update($linkHeap, link, TransientLink#target, Map#Build($linkHeap[link, TransientLink#target], key, val));
+	assume $IsGoodHeap($linkHeap);
+	newStk := Seq#Take(stk, Seq#Length(stk)-3);
+}
+
+procedure NTransientLink#getSourceElement
+	(stk: Seq BoxType, link: ref, key: String) 
+returns 
+	(newStk: Seq BoxType)
+  requires Seq#Length(stk) >= 2; 
+  requires $Unbox(Seq#Index(stk, Seq#Length(stk)-1)):String == key;
+  requires $Unbox(Seq#Index(stk, Seq#Length(stk)-2)):ref == link;
+  requires dtype(link) == Native$TransientLink;
+  ensures newStk == Seq#Build(Seq#Take(stk, Seq#Length(stk)-2), $Box(Map#Elements($linkHeap[link, TransientLink#source])[key]));
+{
+	newStk := Seq#Build(Seq#Take(stk, Seq#Length(stk)-2), $Box(Map#Elements($linkHeap[link, TransientLink#source])[key]));
+}
+
+procedure NTransientLink#getTargetElement
+	(stk: Seq BoxType, link: ref, key: String) 
+returns 
+	(newStk: Seq BoxType)
+  requires Seq#Length(stk) >= 2; 
+  requires $Unbox(Seq#Index(stk, Seq#Length(stk)-1)):String == key;
+  requires $Unbox(Seq#Index(stk, Seq#Length(stk)-2)):ref == link;
+  requires dtype(link) == Native$TransientLink; 
+  ensures newStk == Seq#Build(Seq#Take(stk, Seq#Length(stk)-2), $Box(Map#Elements($linkHeap[link, TransientLink#target])[key]));
+{
+	newStk := Seq#Build(Seq#Take(stk, Seq#Length(stk)-2), $Box(Map#Elements($linkHeap[link, TransientLink#target])[key]));
+}
+
 procedure ASM#Resolve<alpha>(stk: Seq BoxType, heap: HeapType, e: alpha) returns (newStk: Seq BoxType);
   requires $Unbox(Seq#Index(stk, Seq#Length(stk)-2)) == Asm;
   ensures newStk == Seq#Build(
 	Seq#Take(stk, Seq#Length(stk)-2), 
 	ASM#Resolve#Sem($Unbox(Seq#Index(stk, Seq#Length(stk)-2)), heap, e)
-	
 	);
-  
-  
-  // ensures  (typeof(e) == Type#String) ==> newStk == Seq#Build(Seq#Take(stk, Seq#Length(stk)-2), Seq#Index(stk, Seq#Length(stk)-1));
-  // ensures  (typeof(e) == Type#Integer) ==> newStk == Seq#Build(Seq#Take(stk, Seq#Length(stk)-2), Seq#Index(stk, Seq#Length(stk)-1));
-  // ensures  (typeof(e) == Type#Boolean) ==> newStk == Seq#Build(Seq#Take(stk, Seq#Length(stk)-2), Seq#Index(stk, Seq#Length(stk)-1));
-  // ensures  isTarElem(e) ==> newStk == Seq#Build(Seq#Take(stk, Seq#Length(stk)-2), Seq#Index(stk, Seq#Length(stk)-1));
-  // ensures ... when isSrcElem ...
-  // ensures ... when isCollection ...
-  
 
-// this must place before the declaration of __apply...
-// Lemma to prove: ASM#Resolve#Sem(asm, heap, elem) == ASM#Resolve#Sem(asm, oldheap, elem)
-// 		The prove followed by induction on the type of resolve element:  
-//1. the primitive type is straightforward, since the output didnt rely on the heap. 
-//2. The simple ref did not rely on heap neither.
-//3. - The bound between link is sourceElements is fixed, and there is no legal ASM operation would break this. 
-//	 - The bound between link is targetElements is fixed, and there is no legal ASM operation would break this. 
-//	 	==> 
-//		the target ref that from a link is the same between the heap and old heap.
 function ASM#Resolve#Sem<alpha>(this: ref, heap: HeapType, elem: alpha) : BoxType;
-  // axiom (forall this: ref, h: HeapType, anyINT: int :: 
-	// (this == Asm) ==>
-		// (ASM#Resolve#Sem(this, h, anyINT) == anyINT)
-  // );
-  // axiom (forall this: ref, h: HeapType, anyBOOL: bool :: 
-	// (this == Asm) ==>
-		// (ASM#Resolve#Sem(this, h, anyBOOL) == anyBOOL)
-  // );
-  // axiom (forall this: ref, h: HeapType, anySTRING: String :: 
-	// (this == Asm) ==>
-		// (ASM#Resolve#Sem(this, h, anySTRING) == anySTRING)
-  // );
-  // axiom (forall this: ref, h: HeapType, anyREF: ref :: 
-	// (this == Asm && (NTransientLinkSet#getLinkBySourceElement(h, anyREF) == null)) ==>
-		// (ASM#Resolve#Sem(this, h, anyREF) == anyREF)
-  // );
-  // axiom (forall this: ref, h: HeapType, anyREF: ref :: 
-	// (this == Asm && (NTransientLinkSet#getLinkBySourceElement(h, anyREF) != null)) ==>
-		// (ASM#Resolve#Sem(this, h, anyREF) == NTransientLink#getTargetFromSource(
-			// h, NTransientLinkSet#getLinkBySourceElement(h, anyREF), anyREF)
-		// )
-  // );
-  // axiom (forall this: ref, h: HeapType, anyCOL: [int]ref :: 
-	// (this == Asm) ==>
-		// (forall i: int :: (ASM#Resolve#Sem(this, h, anyCOL): [int] ref)[i] == ASM#Resolve#Sem(this, h, anyCOL[i]))
-  // );  
+	axiom (forall this:ref, heap: HeapType, elem: String ::
+		ASM#Resolve#Sem(this, heap, elem) == $Box(elem)
+	);
+	
+	
+function invisble#getLinkbySources(s: Set ref): ref;
+  axiom (forall s1,s2 : Set ref :: !Set#Equal(s1,s2) ==> 
+	invisble#getLinkbySources(s1) != invisble#getLinkbySources(s2));
+	
+/* ------------------------------------------------------ */ 
 
-
-// this information is comes from the ATL rules, but the axiom should be true all the time...
-// the function return null when the src is null, or the isTarElem(src) is true.
-function NTransientLinkSet#getLinkBySourceElement(heap: HeapType, src: ref): ref;
-  // Transitivity 
-  axiom (forall<alpha> l: ref, f: Field (Map String ref), h1, h2: HeapType, mName: String :: 
-	(Map#Elements(h1[l, f])[mName] == Map#Elements(h2[l, f])[mName]) ==>
-		NTransientLinkSet#getLinkBySourceElement(h1, Map#Elements(h1[l, f])[mName]) == NTransientLinkSet#getLinkBySourceElement(h2, Map#Elements(h2[l, f])[mName])
-  );
-// the actual output is comes from the ATL rules - the first output of a ATL rule
-// ps: the third parameter seems not necessary...
-function NTransientLink#getTargetFromSource(heap: HeapType, link: ref, src: ref): ref;
-
-function NTransientLinkSet#getLinksByRule(h: HeapType, rName: String): Seq ref;
-  axiom (forall h:HeapType, rName:String, i,j: int :: 
-	( (0<=i && i<Seq#Length(NTransientLinkSet#getLinksByRule(h, rName))) && 
-	  (i+1<=j && j<Seq#Length(NTransientLinkSet#getLinksByRule(h, rName))) ) ==>
-		Seq#Index(NTransientLinkSet#getLinksByRule(h, rName),i) != Seq#Index(NTransientLinkSet#getLinksByRule(h, rName),j)
-  );
-  axiom (forall h:HeapType, rName:String, i,j: int :: 
-	( 0<=i && i<Seq#Length(NTransientLinkSet#getLinksByRule(h, rName)) ) ==>
-		( ValidLink(h, Seq#Index(NTransientLinkSet#getLinksByRule(h, rName),i)) &&
-		  h[Seq#Index(NTransientLinkSet#getLinksByRule(h, rName),i), TransientLink#rule] == rName )
-  ); 
-// if two rule name is different, they return disjoint result 
-
-
-function Fun#LIB#AllInstanceFrom(h:HeapType, t: TName): Seq ref;
+function Fun#LIB#AllInstanceFrom(h:HeapType, t: ClassName): Seq ref;
   // the length of the return result is >=0; can be useful for termination proof.
-  axiom (forall h:HeapType, t: TName :: 
+  axiom (forall h:HeapType, t: ClassName :: 
     Seq#Length(Fun#LIB#AllInstanceFrom(h, t)) >= 0
   ); 
   // all the model elements contained by the return result are of type $t$.
-  axiom (forall h:HeapType, t: TName, i:int :: 
+  axiom (forall h:HeapType, t: ClassName, i:int :: 
 	( 0<=i && i<Seq#Length(Fun#LIB#AllInstanceFrom(h,t)) ) ==> 
-		typeof( Seq#Index(Fun#LIB#AllInstanceFrom(h,t),i) ) == t
+		dtype( Seq#Index(Fun#LIB#AllInstanceFrom(h,t),i) ) == t
   );
   // all the model elements contained by the return result are allocated
-  axiom (forall h:HeapType, t: TName, i:int :: 
+  axiom (forall h:HeapType, t: ClassName, i:int :: 
 	( 0<=i && i<Seq#Length(Fun#LIB#AllInstanceFrom(h,t)) ) ==> 
-		h[Seq#Index(Fun#LIB#AllInstanceFrom(h,t),i), alloc] 
+		h[Seq#Index(Fun#LIB#AllInstanceFrom(h,t),i), alloc] && Seq#Index(Fun#LIB#AllInstanceFrom(h,t),i) != null
   );
   // all the allocated ref that of type $t$ are contained by the return result. 
-  axiom (forall h:HeapType, o: ref, t: TName :: 
-	(h[o, alloc] && (typeof(o) == t)) ==>
+  axiom (forall h:HeapType, o: ref, t: ClassName :: 
+	(h[o, alloc] && (dtype(o) == t)) ==>
 		Seq#Contains(Fun#LIB#AllInstanceFrom(h,t),o)
   );
   // all the model elements contained by the return result are unique 
-  axiom (forall h:HeapType, t: TName, i,j:int :: 
+  axiom (forall h:HeapType, t: ClassName, i,j:int :: 
     ( (0<=i && i<Seq#Length(Fun#LIB#AllInstanceFrom(h, t))) && 
 	  (i+1<=j && j<Seq#Length(Fun#LIB#AllInstanceFrom(h, t))) ) ==>
 		Seq#Index(Fun#LIB#AllInstanceFrom(h, t),i) != Seq#Index(Fun#LIB#AllInstanceFrom(h, t),j)
   ); 
   
  
- 
-// Sig: TName.allInstanceFrom(In/out model)
-// the top of the stack is IN/OUT, the second top is a TName.
 procedure LIB#AllInstanceFrom(stk: Seq BoxType, h: HeapType) returns (newStk: Seq BoxType, res: Seq ref);
   ensures res == Fun#LIB#AllInstanceFrom(h, $Unbox(Seq#Index(stk, Seq#Length(stk)-2)));
   ensures newStk == Seq#Build(Seq#Take(stk, Seq#Length(stk)-2), $Box(res));
  
-  
+ 
+ 
+ 
+ 
+/* h refers to linkheap, r referes to the rule name */
+function NTransientLinkSet#getLinksByRule(h:HeapType, rule: String): Seq ref;
+  // the length of the return result is >=0; can be useful for termination proof.
+  axiom (forall h:HeapType, r: String :: 
+    Seq#Length(NTransientLinkSet#getLinksByRule(h, r)) >= 0
+  ); 
+  // unique links
+  axiom (forall h:HeapType, r: String, i,j:int :: 
+    ( (0<=i && i<Seq#Length(NTransientLinkSet#getLinksByRule(h,r))) && 
+	  (i+1<=j && j<Seq#Length(NTransientLinkSet#getLinksByRule(h,r)) ) ==>
+		Seq#Index(NTransientLinkSet#getLinksByRule(h, r),i) != Seq#Index(NTransientLinkSet#getLinksByRule(h, r),j)
+  ));
+  // unique target elements
+  axiom (forall h:HeapType, r: String, i,j:int :: 
+    ( (0<=i && i<Seq#Length(NTransientLinkSet#getLinksByRule(h,r))) && 
+	  (i+1<=j && j<Seq#Length(NTransientLinkSet#getLinksByRule(h,r)) ) ==>
+		getTarsBySrcs(Seq#Singleton(Map#Elements(read(h, Seq#Index(NTransientLinkSet#getLinksByRule(h, r),i), TransientLink#source))[_s])) != getTarsBySrcs(Seq#Singleton(Map#Elements(read(h, Seq#Index(NTransientLinkSet#getLinksByRule(h, r),j), TransientLink#source))[_s]))
+  ));
+  // all links's src and target are paired
+  axiom (forall h:HeapType, r: String, i: int:: 0<=i &&i <Seq#Length(NTransientLinkSet#getLinksByRule(h,r)) ==>			
+			getTarsBySrcs(Seq#Singleton(Map#Elements(h[Seq#Index(NTransientLinkSet#getLinksByRule(h,r),i), TransientLink#source])[_s])) == 
+			Map#Elements(h[Seq#Index(NTransientLinkSet#getLinksByRule(h,r),i), TransientLink#target])[_t]
+		);
+		
 //--------------------------------
 //-------- Helper Function -------
 //--------------------------------
-
-function typeof<alpha>(alpha): TName;
-  axiom (forall s: String :: typeof(s) == Type#String);
-  axiom (forall i: int :: typeof(i) == Type#Integer);
-  axiom (forall b: bool :: typeof(b) == Type#Boolean);
- 
-  
-  
-function toString(ref): String;
-
-function isFullyAllocated(o: ref): bool;
-
-function isTarElem<alpha>(e: alpha): bool;
-
-function ValidLink(Heap: HeapType, l: ref): bool
-{
-	Heap[l, alloc] &&
-	typeof(l) == Native$TransientLink 
-}
-
-const unique proc: Field bool;
-
 
 function top(Seq BoxType): BoxType;
   axiom (forall stk: Seq BoxType :: top(stk) == Seq#Index(stk, Seq#Length(stk)-1));
 
 function isSrcRef(ref) : bool;
-  axiom (forall o: ref :: (typeof(o)==ER$ERSchema || typeof(o) == ER$ERAttribute || typeof(o) == ER$Entity) <==> isSrcRef(o));
+  axiom (forall o: ref :: (dtype(o)==ER$ERSchema || dtype(o) == ER$ERAttribute || dtype(o) == ER$Entity) <==> isSrcRef(o));
   
 function getSrcLink(ref): ref;
-  axiom (forall o1,o2:ref :: o1 == o2 && isSrcRef(o1) ==> (getSrcLink(o1) == getSrcLink(o2) && typeof(getSrcLink(o1)) == Native$TransientLink ));
+  axiom (forall o1,o2:ref :: o1 == o2 && isSrcRef(o1) ==> (getSrcLink(o1) == getSrcLink(o2) && dtype(getSrcLink(o1)) == Native$TransientLink ));
   
-axiom (forall o1,o2: ref :: o1 == o2 ==> typeof(o1) == typeof(o2));
+axiom (forall o1,o2: ref :: o1 == o2 ==> dtype(o1) == dtype(o2));
