ATL-Correctness/ER2REL_Correctness.bpl
@@ -1,0 +1,326 @@
+procedure driver()
+  requires valid_src_model($srcHeap);
+  // ERSchema1 != ERSchema2 ==> ERSchema1.name != ERSchema2.name
+  requires (forall $i1, $i2: ref :: $i1!=$i2 && $i1!=null && read($srcHeap, $i1, alloc) && dtype($i1) == ER$ERSchema
+				&& $i2!=null && read($srcHeap, $i2, alloc) && dtype($i2) == ER$ERSchema ==>
+				read($srcHeap, $i1, ERSchema.name) != read($srcHeap, $i2, ERSchema.name));
+  // ERSchema.alloc ==> 0<=j1<j2<ERSchema1.entities.len ==> ERSchema1.entities[j1].name != ERSchema1.entities[j2].name
+  requires (forall r: ref :: r!=null && read($srcHeap, r, alloc) && dtype(r) == ER$ERSchema ==> 
+			( forall j1,j2: int :: 0<=j1 && j1<j2 && j2<_System.array.Length(read($srcHeap, r, ERSchema.entities))  ==>
+				// [todo]prevent aliasing, supposed to put in valid model 
+				$Unbox(read($srcHeap, read($srcHeap, r, ERSchema.entities), IndexField(j1))): ref != $Unbox(read($srcHeap, read($srcHeap, r, ERSchema.entities), IndexField(j2))): ref ==>
+				read($srcHeap, $Unbox(read($srcHeap, read($srcHeap, r, ERSchema.entities), IndexField(j1))), Entity.name) != read($srcHeap, $Unbox(read($srcHeap, read($srcHeap, r, ERSchema.entities), IndexField(j2))), Entity.name)
+			));
+  // ERSchema.alloc ==> 0<=j1<j2<ERSchema1.relships.len ==> ERSchema1.relships[j1].name != ERSchema1.relships[j2].name
+  requires (forall r: ref :: r!=null && read($srcHeap, r, alloc) && dtype(r) == ER$ERSchema ==> 
+			( forall j1,j2: int :: 0<=j1 && j1<j2 && j2<_System.array.Length(read($srcHeap, r, ERSchema.relships))  ==>
+				// [todo]prevent aliasing, supposed to put in valid model 
+				$Unbox(read($srcHeap, read($srcHeap, r, ERSchema.relships), IndexField(j1))): ref != $Unbox(read($srcHeap, read($srcHeap, r, ERSchema.relships), IndexField(j2))): ref ==>
+				read($srcHeap, $Unbox(read($srcHeap, read($srcHeap, r, ERSchema.relships), IndexField(j1))), Relship.name) != read($srcHeap, $Unbox(read($srcHeap, read($srcHeap, r, ERSchema.relships), IndexField(j2))), Relship.name)
+			));
+  // ERSchema.alloc ==> 0<=i<ERSchema.entities.len && 0<=j<ERSchema.relships.len ==> ERSchema.entities[i].name != ERSchema.relships[j].name
+  requires (forall r: ref :: r!=null && read($srcHeap, r, alloc) && dtype(r) == ER$ERSchema ==> 
+			( forall i: int :: 0<=i && i<_System.array.Length(read($srcHeap, r, ERSchema.entities))  ==>
+			 ( forall j: int :: 0<=j && j<_System.array.Length(read($srcHeap, r, ERSchema.relships))  ==>
+				$Unbox(read($srcHeap, read($srcHeap, r, ERSchema.entities), IndexField(i))): ref != $Unbox(read($srcHeap, read($srcHeap, r, ERSchema.relships), IndexField(j))): ref ==>
+				read($srcHeap, $Unbox(read($srcHeap, read($srcHeap, r, ERSchema.entities), IndexField(i))), Entity.name) != read($srcHeap, $Unbox(read($srcHeap, read($srcHeap, r, ERSchema.relships), IndexField(j))), Relship.name)
+			)));
+  modifies $tarHeap,$linkHeap;
+  ensures (forall $o1, $o2: ref :: $o1!=$o2 && $o1!=null && read($tarHeap, $o1, alloc) && dtype($o1) == REL$RELSchema
+				&& $o2!=null && read($tarHeap, $o2, alloc) && dtype($o2) == REL$RELSchema ==>
+				read($tarHeap, $o1, RELSchema.name) != read($tarHeap, $o2, RELSchema.name));  
+  ensures (forall $o: ref :: {read($tarHeap, $o, alloc)} $o!=null && read($tarHeap, $o, alloc) && dtype($o) == REL$RELSchema ==> 
+			( forall j1,j2: int :: {$Unbox(read($tarHeap, read($tarHeap, $o, RELSchema.relations), IndexField(j1))): ref, $Unbox(read($tarHeap, read($tarHeap, $o, RELSchema.relations), IndexField(j2))): ref} 
+			   0<=j1 && j1<j2 && j2<_System.array.Length(read($tarHeap, $o, RELSchema.relations))  ==>
+				$Unbox(read($tarHeap, read($tarHeap, $o, RELSchema.relations), IndexField(j1))): ref != $Unbox(read($tarHeap, read($tarHeap, $o, RELSchema.relations), IndexField(j2))): ref ==>
+					read($tarHeap, $Unbox(read($tarHeap, read($tarHeap, $o, RELSchema.relations), IndexField(j1))), Relation.name) != read($tarHeap, $Unbox(read($tarHeap, read($tarHeap, $o, RELSchema.relations), IndexField(j2))), Relation.name)	
+			));		
+{
+	
+	var hp: HeapType  where $IsGoodHeap(hp);
+
+
+	
+
+	call init_tar_model(); 
+	
+
+	call S2S_match();
+	call E2R_match();
+	call R2R_match();
+	call EA2A_match();
+	call RA2A_match();
+	call RA2AK_match();
+
+
+
+	call S2S_applys();
+	call E2R_applys();
+	call R2R_applys();
+
+// helper: to better explain the layout of RELSchema.relations
+assert (forall r: ref :: r!=null && read($srcHeap, r, alloc) && dtype(r) == ER$ERSchema ==> 
+			( forall j: int :: _System.array.Length(read($srcHeap, r, ERSchema.entities))<=j && j<_System.array.Length(read($tarHeap, getTarsBySrcs(Seq#Singleton(r)), RELSchema.relations))  ==>
+				read($tarHeap, $Unbox(read($tarHeap, read($tarHeap, getTarsBySrcs(Seq#Singleton(r)), RELSchema.relations), IndexField(j))), Relation.name) == read($srcHeap, $Unbox(read($srcHeap, read($srcHeap, r, ERSchema.relships), IndexField(j-_System.array.Length(read($srcHeap, r, ERSchema.entities))))), Relship.name)
+			));	
+			
+
+
+/*
+// sanity check, redundant
+assert (forall r: ref :: r!=null && read($srcHeap, r, alloc) && dtype(r) == ER$ERSchema ==> 
+			( forall j: int :: 0<=j && j<_System.array.Length(read($tarHeap, getTarsBySrcs(Seq#Singleton(r)), RELSchema.relations))  ==>
+				read($tarHeap, $Unbox(read($tarHeap, read($tarHeap, getTarsBySrcs(Seq#Singleton(r)), RELSchema.relations), IndexField(j))), Relation.name) == read($srcHeap, $Unbox(read($srcHeap, read($srcHeap, r, ERSchema.entities), IndexField(j))), Entity.name)
+			));	
+assert (forall r: ref :: r!=null && read($srcHeap, r, alloc) && dtype(r) == ER$ERSchema ==> 
+			( forall j: int :: 0<=j && j<_System.array.Length(read($srcHeap, r, ERSchema.relships))  ==>
+				read($tarHeap, $Unbox(read($tarHeap, read($tarHeap, getTarsBySrcs(Seq#Singleton(r)), RELSchema.relations), IndexField(j+_System.array.Length(read($srcHeap, r, ERSchema.entities))))), Relation.name) == read($srcHeap, $Unbox(read($srcHeap, read($srcHeap, r, ERSchema.relships), IndexField(j))), Relship.name)
+			));	
+*/
+
+	
+}
+
+// the outcome of init is that: no rule to handle src tuple in ATL spec will return null, or not allocated yet.
+procedure init_tar_model();
+modifies $tarHeap;
+ensures  (forall $o: ref :: $o == null || !read($tarHeap, $o, alloc));
+
+
+procedure S2S_match();
+requires (forall $i: ref :: $i!=null && read($srcHeap, $i, alloc) && dtype($i) == ER$ERSchema ==> 
+		getTarsBySrcs(Seq#Singleton($i))==null || !read($tarHeap, getTarsBySrcs(Seq#Singleton($i)), alloc));
+modifies $tarHeap,$linkHeap;
+ensures (forall $i: ref :: $i!=null && read($srcHeap, $i, alloc) && dtype($i) == ER$ERSchema ==> 
+		getTarsBySrcs(Seq#Singleton($i))!=null && read($tarHeap, getTarsBySrcs(Seq#Singleton($i)), alloc));
+ensures (forall<alpha> $o : ref, $f: Field alpha ::
+	($o == null || read($tarHeap, $o, $f) == read(old($tarHeap), $o, $f) || (dtype($o) == REL$RELSchema && dtype(Seq#Index(getTarsBySrcs_inverse($o), 0)) == ER$ERSchema && $f==alloc)));
+free ensures $HeapSucc(old($tarHeap), $tarHeap);
+free ensures $HeapSucc(old($linkHeap), $linkHeap);
+free ensures surj_tar_model($srcHeap, $tarHeap);
+
+procedure E2R_match();
+requires (forall $i: ref :: $i!=null && read($srcHeap, $i, alloc) && dtype($i) == ER$Entity ==> 
+		getTarsBySrcs(Seq#Singleton($i))==null || !read($tarHeap, getTarsBySrcs(Seq#Singleton($i)), alloc));
+modifies $tarHeap,$linkHeap;
+ensures (forall $i: ref :: $i!=null && read($srcHeap, $i, alloc) && dtype($i) == ER$Entity ==> 
+		getTarsBySrcs(Seq#Singleton($i))!=null && read($tarHeap, getTarsBySrcs(Seq#Singleton($i)), alloc));
+ensures (forall<alpha> $o : ref, $f: Field alpha ::
+	($o == null || read($tarHeap, $o, $f) == read(old($tarHeap), $o, $f) || (dtype($o) == REL$Relation && dtype(Seq#Index(getTarsBySrcs_inverse($o), 0)) == ER$Entity && $f==alloc)));
+free ensures $HeapSucc(old($tarHeap), $tarHeap);
+free ensures $HeapSucc(old($linkHeap), $linkHeap);
+free ensures surj_tar_model($srcHeap, $tarHeap);
+
+procedure R2R_match();
+requires (forall $i: ref :: $i!=null && read($srcHeap, $i, alloc) && dtype($i) == ER$Relship ==> 
+		getTarsBySrcs(Seq#Singleton($i))==null || !read($tarHeap, getTarsBySrcs(Seq#Singleton($i)), alloc));
+modifies $tarHeap,$linkHeap;
+ensures (forall $i: ref :: $i!=null && read($srcHeap, $i, alloc) && dtype($i) == ER$Relship ==> 
+		getTarsBySrcs(Seq#Singleton($i))!=null && read($tarHeap, getTarsBySrcs(Seq#Singleton($i)), alloc));
+ensures (forall<alpha> $o : ref, $f: Field alpha ::
+	($o == null || read($tarHeap, $o, $f) == read(old($tarHeap), $o, $f) || (dtype($o) == REL$Relation && dtype(Seq#Index(getTarsBySrcs_inverse($o), 0)) == ER$Relship && $f==alloc)));
+free ensures $HeapSucc(old($tarHeap), $tarHeap);
+free ensures $HeapSucc(old($linkHeap), $linkHeap);
+free ensures surj_tar_model($srcHeap, $tarHeap);
+
+procedure EA2A_match();
+requires (forall att: ref :: att!=null && read($srcHeap, att, alloc) && dtype(att) == ER$ERAttribute ==> 
+			(forall ent: ref :: ent!=null && read($srcHeap, ent, alloc) && dtype(ent) == ER$Entity ==> 
+				$srcHeap[att, ERAttribute.entity] == ent ==>
+				getTarsBySrcs(Seq#Build(Seq#Singleton(att),ent))==null || !read($tarHeap, getTarsBySrcs(Seq#Build(Seq#Singleton(att),ent)), alloc)));
+modifies $tarHeap,$linkHeap;
+ensures (forall att: ref :: att!=null && read($srcHeap, att, alloc) && dtype(att) == ER$ERAttribute ==> 
+			 (forall ent: ref :: ent!=null && read($srcHeap, ent, alloc) && dtype(ent) == ER$Entity ==> 
+				$srcHeap[att, ERAttribute.entity] == ent ==>
+				getTarsBySrcs(Seq#Build(Seq#Singleton(att),ent))!=null && read($tarHeap, getTarsBySrcs(Seq#Build(Seq#Singleton(att),ent)), alloc)));
+ensures (forall<alpha> $o : ref, $f: Field alpha ::
+	($o == null || read($tarHeap, $o, $f) == read(old($tarHeap), $o, $f) || (dtype($o) == REL$RELAttribute && dtype(Seq#Index(getTarsBySrcs_inverse($o), 0)) == ER$ERAttribute && dtype(Seq#Index(getTarsBySrcs_inverse($o), 1)) == ER$Entity && $f==alloc)));
+free ensures $HeapSucc(old($tarHeap), $tarHeap);
+free ensures $HeapSucc(old($linkHeap), $linkHeap);
+free ensures surj_tar_model($srcHeap, $tarHeap);
+
+procedure RA2A_match();
+requires (forall att: ref :: att!=null && read($srcHeap, att, alloc) && dtype(att) == ER$ERAttribute ==> 
+			(forall ent: ref :: ent!=null && read($srcHeap, ent, alloc) && dtype(ent) == ER$Relship ==> 
+				$srcHeap[att, ERAttribute.relship] == ent ==>
+				getTarsBySrcs(Seq#Build(Seq#Singleton(att),ent))==null || !read($tarHeap, getTarsBySrcs(Seq#Build(Seq#Singleton(att),ent)), alloc)));
+modifies $tarHeap,$linkHeap;
+ensures (forall att: ref :: att!=null && read($srcHeap, att, alloc) && dtype(att) == ER$ERAttribute ==> 
+			 (forall ent: ref :: ent!=null && read($srcHeap, ent, alloc) && dtype(ent) == ER$Relship ==> 
+				$srcHeap[att, ERAttribute.relship] == ent ==>
+				getTarsBySrcs(Seq#Build(Seq#Singleton(att),ent))!=null && read($tarHeap, getTarsBySrcs(Seq#Build(Seq#Singleton(att),ent)), alloc)));
+ensures (forall<alpha> $o : ref, $f: Field alpha ::
+	($o == null || read($tarHeap, $o, $f) == read(old($tarHeap), $o, $f) || (dtype($o) == REL$RELAttribute && dtype(Seq#Index(getTarsBySrcs_inverse($o), 0)) == ER$ERAttribute && dtype(Seq#Index(getTarsBySrcs_inverse($o), 1)) == ER$Relship && $f==alloc)));
+free ensures $HeapSucc(old($tarHeap), $tarHeap);
+free ensures $HeapSucc(old($linkHeap), $linkHeap);
+free ensures surj_tar_model($srcHeap, $tarHeap);
+
+procedure RA2AK_match();
+requires (forall att: ref :: att!=null && read($srcHeap, att, alloc) && dtype(att) == ER$ERAttribute ==> 
+			(forall rse: ref :: rse!=null && read($srcHeap, rse, alloc) && dtype(rse) == ER$RelshipEnd ==> 
+				($srcHeap[att, ERAttribute.entity] == $srcHeap[rse, RelshipEnd.entity] && $srcHeap[att, ERAttribute.isKey]) ==>
+					getTarsBySrcs(Seq#Build(Seq#Singleton(att),rse))==null || !read($tarHeap, getTarsBySrcs(Seq#Build(Seq#Singleton(att),rse)), alloc)));
+modifies $tarHeap,$linkHeap;
+ensures (forall att: ref :: att!=null && read($srcHeap, att, alloc) && dtype(att) == ER$ERAttribute ==> 
+			 (forall rse: ref :: rse!=null && read($srcHeap, rse, alloc) && dtype(rse) == ER$RelshipEnd ==> 
+				($srcHeap[att, ERAttribute.entity] == $srcHeap[rse, RelshipEnd.entity] && $srcHeap[att, ERAttribute.isKey]) ==>
+					getTarsBySrcs(Seq#Build(Seq#Singleton(att),rse))!=null && read($tarHeap, getTarsBySrcs(Seq#Build(Seq#Singleton(att),rse)), alloc)));
+ensures (forall<alpha> $o : ref, $f: Field alpha ::
+	($o == null || read($tarHeap, $o, $f) == read(old($tarHeap), $o, $f) || (dtype($o) == REL$RELAttribute && dtype(Seq#Index(getTarsBySrcs_inverse($o), 0)) == ER$ERAttribute && dtype(Seq#Index(getTarsBySrcs_inverse($o), 1)) == ER$RelshipEnd && $f==alloc)));
+free ensures $HeapSucc(old($tarHeap), $tarHeap);
+free ensures $HeapSucc(old($linkHeap), $linkHeap);
+free ensures surj_tar_model($srcHeap, $tarHeap);
+
+procedure S2S_applys();
+requires (forall r: ref :: r!=null && read($srcHeap, r, alloc) && dtype(r) == ER$ERSchema ==>
+		read($tarHeap, getTarsBySrcs(Seq#Singleton(r)), alloc) 
+	 && getTarsBySrcs(Seq#Singleton(r)) != null 
+	 && dtype(getTarsBySrcs(Seq#Singleton(r))) == REL$RELSchema	);
+modifies $tarHeap;
+// t.name <- s.name
+ensures (forall r: ref :: r!=null && read($srcHeap, r, alloc) && dtype(r) == ER$ERSchema ==> 
+		read($tarHeap, getTarsBySrcs(Seq#Singleton(r)), RELSchema.name) == read($srcHeap, r, ERSchema.name));
+// dtype(t.relations) = class._System.array
+ensures (forall r: ref :: r!=null && read($srcHeap, r, alloc) && dtype(r) == ER$ERSchema ==> 
+	dtype(read($tarHeap, getTarsBySrcs(Seq#Singleton(r)), RELSchema.relations)) == class._System.array
+);	
+// t.relations != null && t.relations.alloc
+ensures (forall r: ref :: r!=null && read($srcHeap, r, alloc) && dtype(r) == ER$ERSchema ==> 
+	read($tarHeap, getTarsBySrcs(Seq#Singleton(r)), RELSchema.relations) != null 
+ && read($tarHeap, read($tarHeap, getTarsBySrcs(Seq#Singleton(r)), RELSchema.relations), alloc)
+);
+// length(t.relations) = length(s.entities)+length(s.relships)
+ensures (forall r: ref :: r!=null && read($srcHeap, r, alloc) && dtype(r) == ER$ERSchema ==> 
+		_System.array.Length(read($tarHeap, getTarsBySrcs(Seq#Singleton(r)), RELSchema.relations)) 
+	 == _System.array.Length(read($srcHeap, r, ERSchema.entities))+_System.array.Length(read($srcHeap, r, ERSchema.relships))
+);
+// t.relations[j] != null t.relations[j].alloc && dtype(t.relations[j]) == REL$Relation
+ensures (forall r: ref :: r!=null && read($srcHeap, r, alloc) && dtype(r) == ER$ERSchema ==> 
+			( forall j: int :: 0<=j && j<_System.array.Length(read($tarHeap, getTarsBySrcs(Seq#Singleton(r)), RELSchema.relations))  ==>
+				$Unbox(read($tarHeap, read($tarHeap, getTarsBySrcs(Seq#Singleton(r)), RELSchema.relations), IndexField(j))): ref != null
+			 &&	read($tarHeap, $Unbox(read($tarHeap, read($tarHeap, getTarsBySrcs(Seq#Singleton(r)), RELSchema.relations), IndexField(j))): ref, alloc)
+			 && dtype($Unbox(read($tarHeap, read($tarHeap, getTarsBySrcs(Seq#Singleton(r)), RELSchema.relations), IndexField(j))): ref) == REL$Relation
+			));
+// t.relations[j] == s.entities[j]
+ensures (forall r: ref :: r!=null && read($srcHeap, r, alloc) && dtype(r) == ER$ERSchema ==> 
+			( forall j: int :: 0<=j && j<_System.array.Length(read($srcHeap, r, ERSchema.entities))  ==>
+				$Unbox(read($tarHeap, read($tarHeap, getTarsBySrcs(Seq#Singleton(r)), RELSchema.relations), IndexField(j))): ref ==
+				getTarsBySrcs(Seq#Singleton( $Unbox(read($srcHeap, read($srcHeap, r, ERSchema.entities), IndexField(j))): ref) )
+			));
+// t.relations[j+len(s.entities)] == s.relships[j]
+ensures (forall r: ref :: r!=null && read($srcHeap, r, alloc) && dtype(r) == ER$ERSchema ==> 
+			( forall j: int :: 0<=j && j<_System.array.Length(read($srcHeap, r, ERSchema.relships))  ==>
+				$Unbox(read($tarHeap, read($tarHeap, getTarsBySrcs(Seq#Singleton(r)), RELSchema.relations), IndexField(j+_System.array.Length(read($srcHeap, r, ERSchema.entities))))): ref ==
+				getTarsBySrcs(Seq#Singleton( $Unbox(read($srcHeap, read($srcHeap, r, ERSchema.relships), IndexField(j))): ref) )
+			));
+// frame property, i.e. what is changed / not changed.
+// [todo: feel under-specified here] the array element is also changed, effected on field [IndexField], i.e.:
+// (exists k: int :: 0 <= k && k < _System.array.Length([t.relations]) && $o == [t.relations] && $f == IndexField(k))
+ensures (forall<alpha> $o: ref, $f: Field alpha :: 
+	$o != null && read(old($tarHeap), $o, alloc) ==>
+		( (dtype($o) == REL$RELSchema && dtype(Seq#Index(getTarsBySrcs_inverse($o), 0)) == ER$ERSchema && ($f == RELSchema.name || $f == RELSchema.relations)) || (read($tarHeap, $o, $f) == read(old($tarHeap), $o, $f))));
+ensures $HeapSucc(old($tarHeap), $tarHeap);
+free ensures surj_tar_model($srcHeap, $tarHeap);
+		
+/* redundant
+ensures   (forall r: ref :: r!=null && read($srcHeap, r, alloc) && dtype(r) == ER$ERSchema ==>
+				getTarsBySrcs(Seq#Singleton(r)) != null && dtype(getTarsBySrcs(Seq#Singleton(r))) == REL$RELSchema	);
+// this is conveyed by E2R rule.
+ensures (forall r: ref :: r!=null && read($srcHeap, r, alloc) && dtype(r) == ER$ERSchema ==> 
+			( forall j: int :: 0<=j && j<_System.array.Length(read($tarHeap, getTarsBySrcs(Seq#Singleton(r)), RELSchema.relations))  ==>
+				dtype($Unbox(read($tarHeap, read($tarHeap, getTarsBySrcs(Seq#Singleton(r)), RELSchema.relations), IndexField(j))): ref) ==
+				REL$Relation
+			));							
+*/
+
+
+procedure E2R_applys();
+requires (forall r: ref :: r!=null && read($srcHeap, r, alloc) && dtype(r) == ER$Entity ==>
+		read($tarHeap, getTarsBySrcs(Seq#Singleton(r)), alloc) 
+	 && getTarsBySrcs(Seq#Singleton(r)) != null 
+	 && dtype(getTarsBySrcs(Seq#Singleton(r))) == REL$Relation	);
+modifies $tarHeap;
+// t.name <- s.name
+ensures (forall r: ref :: r!=null && read($srcHeap, r, alloc) && dtype(r) == ER$Entity ==> 
+		read($tarHeap, getTarsBySrcs(Seq#Singleton(r)), Relation.name) == read($srcHeap, r, Entity.name));
+// frame property
+ensures (forall<alpha> $o: ref, $f: Field alpha :: 
+	$o != null && read(old($tarHeap), $o, alloc) ==>
+		((dtype($o) == REL$Relation && dtype(Seq#Index(getTarsBySrcs_inverse($o), 0)) == ER$Entity && $f == Relation.name) || (read($tarHeap, $o, $f) == read(old($tarHeap), $o, $f))));
+ensures $HeapSucc(old($tarHeap), $tarHeap);
+free ensures surj_tar_model($srcHeap, $tarHeap);
+
+procedure R2R_applys();
+requires (forall r: ref :: r!=null && read($srcHeap, r, alloc) && dtype(r) == ER$Relship ==>
+		read($tarHeap, getTarsBySrcs(Seq#Singleton(r)), alloc) 
+	 && getTarsBySrcs(Seq#Singleton(r)) != null 
+	 && dtype(getTarsBySrcs(Seq#Singleton(r))) == REL$Relation	);
+modifies $tarHeap;
+// t.name <- s.name
+ensures (forall r: ref :: r!=null && read($srcHeap, r, alloc) && dtype(r) == ER$Relship ==> 
+		read($tarHeap, getTarsBySrcs(Seq#Singleton(r)), Relation.name) == read($srcHeap, r, Relship.name));
+// frame property
+ensures (forall<alpha> $o: ref, $f: Field alpha :: 
+	$o != null && read(old($tarHeap), $o, alloc) ==>
+		((dtype($o) == REL$Relation && dtype(Seq#Index(getTarsBySrcs_inverse($o), 0)) == ER$Relship && $f == Relation.name) || (read($tarHeap, $o, $f) == read(old($tarHeap), $o, $f))));
+ensures $HeapSucc(old($tarHeap), $tarHeap);
+free ensures surj_tar_model($srcHeap, $tarHeap);
+
+/* --------------------------------  */
+
+// [todo]
+// - (forall $i1, $i2: ref :: $i1!=$i2 ==> Seq#Index(getTarsBySrcs_inverse($i1), 0) != Seq#Index(getTarsBySrcs_inverse($i2), 0));	
+function valid_src_model($h: HeapType): bool
+{
+(forall $i: ref ::
+	
+	($i!=null && read($h, $i, alloc) && dtype($i) == ER$ERSchema ==> 
+	 // ER$ERSchema => its [entities] feature is not null, and every of them is type of [ER$Entity], not [null], and is [allocated]
+		( read($h, $i, ERSchema.entities)!=null &&
+		 (forall j: int :: 0<=j && j<_System.array.Length(read($h, $i, ERSchema.entities)) ==> 
+		    ($Unbox(read($h, read($h, $i, ERSchema.entities), IndexField(j))): ref !=null 
+		      && read($h, $Unbox(read($h, read($h, $i, ERSchema.entities), IndexField(j))): ref, alloc)
+		      && dtype($Unbox(read($h, read($h, $i, ERSchema.entities), IndexField(j))): ref)==ER$Entity) ))
+	 // ER$ERSchema => its [relships] feature is not null, and every of them is type of [ER$Relship], not [null], and is [allocated]
+	 && ( read($h, $i, ERSchema.relships)!=null &&
+		 (forall j: int :: 0<=j && j<_System.array.Length(read($h, $i, ERSchema.relships)) ==> 
+		    ($Unbox(read($h, read($h, $i, ERSchema.relships), IndexField(j))): ref !=null 
+		      && read($h, $Unbox(read($h, read($h, $i, ERSchema.relships), IndexField(j))): ref, alloc)
+		      && dtype($Unbox(read($h, read($h, $i, ERSchema.relships), IndexField(j))): ref)==ER$Relship) ))
+	)
+)
+}
+
+
+/* --------------------------------  */
+
+			
+/*
+
+	// less ideal. which quantify over getTarsBySrcs.
+	ensures (forall $i1, $i2: ref :: $i1!=$i2 && $i1!=null && read($srcHeap, $i1, alloc) && dtype($i1) == ER$ERSchema && $i2!=null && read($srcHeap, $i2, alloc) && dtype($i2) == ER$ERSchema ==>
+				read($tarHeap, getTarsBySrcs(Seq#Singleton($i1)), RELSchema.name) != read($tarHeap, getTarsBySrcs(Seq#Singleton($i2)), RELSchema.name));
+		
+	// less ideal
+	ensures (forall r: ref :: r!=null && read($srcHeap, r, alloc) && dtype(r) == ER$ERSchema ==> 
+			( forall j1,j2: int :: 0<=j1 && j1<j2 && j2<_System.array.Length(read($tarHeap, getTarsBySrcs(Seq#Singleton(r)), RELSchema.relations))  ==>
+				$Unbox(read($tarHeap, read($tarHeap, getTarsBySrcs(Seq#Singleton(r)), RELSchema.relations), IndexField(j1))): ref != $Unbox(read($tarHeap, read($tarHeap, getTarsBySrcs(Seq#Singleton(r)), RELSchema.relations), IndexField(j2))): ref ==>
+					read($tarHeap, $Unbox(read($tarHeap, read($tarHeap, getTarsBySrcs(Seq#Singleton(r)), RELSchema.relations), IndexField(j1))), Relation.name) != read($tarHeap, $Unbox(read($tarHeap, read($tarHeap, getTarsBySrcs(Seq#Singleton(r)), RELSchema.relations), IndexField(j2))), Relation.name)
+				
+			));
+			
+// boiler 1			
+ensures (forall<alpha> $o : ref, $f: Field alpha ::
+	($o == null || read($tarHeap, $o, $f) == read(old($tarHeap), $o, $f) || (dtype($o) == REL$RELSchema && dtype(Seq#Index(getTarsBySrcs_inverse($o), 0)) == ER$ERSchema && ($f == RELSchema.name || $f == RELSchema.relations))));
+// boiler 2
+ensures (forall<alpha> $o: ref, $f: Field alpha :: 
+	$o != null && read(old($tarHeap), $o, alloc) ==>
+		((dtype($o) == REL$RELSchema && dtype(Seq#Index(getTarsBySrcs_inverse($o), 0)) == ER$ERSchema && ($f == RELSchema.name || $f == RELSchema.relations)) || (read($tarHeap, $o, $f) == read(old($tarHeap), $o, $f))));
+// boiler 1			
+ensures (forall<alpha> $o : ref, $f: Field alpha ::
+	($o == null || read($tarHeap, $o, $f) == read(old($tarHeap), $o, $f) || (dtype($o) == REL$Relation && dtype(Seq#Index(getTarsBySrcs_inverse($o), 0)) == ER$Entity && ($f == Relation.name))));		
+// boiler 2	
+ensures (forall<alpha> $o: ref, $f: Field alpha :: 
+	$o != null && read(old($tarHeap), $o, alloc) ==>
+		((dtype($o) == REL$Relation && dtype(Seq#Index(getTarsBySrcs_inverse($o), 0)) == ER$Entity && $f == Relation.name) || (read($tarHeap, $o, $f) == read(old($tarHeap), $o, $f))));		
+*/
