Generated/MATCH_S2S.bpl
@@ -1,0 +1,154 @@
+/*
+rule S2S { 
+  from s : ER!ERSchema to t : REL!RELSchema ( name  <- s.name, relations <-s.entities, relations <-s.relships)}
+*/
+
+
+
+procedure S2S_match();
+requires (forall $i: ref :: $i!=null && read($srcHeap, $i, alloc) && dtype($i) == ER$ERSchema ==> 
+		getTarsBySrcs(Seq#Singleton($i))==null || !read($tarHeap, getTarsBySrcs(Seq#Singleton($i)), alloc));
+modifies $tarHeap,$linkHeap;
+ensures (forall $i: ref :: $i!=null && read($srcHeap, $i, alloc) && dtype($i) == ER$ERSchema ==> 
+		getTarsBySrcs(Seq#Singleton($i))!=null && read($tarHeap, getTarsBySrcs(Seq#Singleton($i)), alloc));
+ensures (forall<alpha> $o : ref, $f: Field alpha ::
+	($o == null || read($tarHeap, $o, $f) == read(old($tarHeap), $o, $f) || (dtype($o) == REL$RELSchema && dtype(Seq#Index(getTarsBySrcs_inverse($o), 0)) == ER$ERSchema && $f==alloc)));
+free ensures $HeapSucc(old($tarHeap), $tarHeap);
+free ensures $HeapSucc(old($linkHeap), $linkHeap);
+free ensures surj_tar_model($srcHeap, $tarHeap);
+
+implementation S2S_match () returns ()
+{
+
+var stk: Seq BoxType;
+var $i: int;
+var s: ref;	//slot: 1
+var self: ref;	//slot: 0
+var obj#4: Seq ref;
+var obj#11: ref;
+var obj#23: ref;
+
+
+stk := OpCode#Aux#InitStk();
+
+
+call stk := OpCode#Push(stk, _ERSchema);
+call stk := OpCode#Push(stk, _ER);
+call stk := OpCode#Findme(stk);
+call stk := OpCode#Push(stk, _IN);
+call stk, obj#4 := LIB#AllInstanceFrom(stk, $srcHeap);
+
+
+assert (forall i: ref :: i!=null && read($srcHeap, i, alloc) && dtype(i) == ER$ERSchema ==> Seq#Contains(obj#4,i)); // test contaiment of allinstance function
+
+
+
+
+$i:=0;
+call stk := OpCode#Pop(stk);
+while($i<Seq#Length(obj#4))
+  invariant $i<=Seq#Length(obj#4);
+  invariant (forall i: int:: 0<=i &&i <$i ==>
+			true ==>
+			(
+				Seq#Index(obj#4,i)!=null && read($srcHeap, Seq#Index(obj#4,i), alloc) && dtype(Seq#Index(obj#4,i)) == ER$ERSchema ==> 
+					getTarsBySrcs(Seq#Singleton(Seq#Index(obj#4,i)))!=null && read($tarHeap, getTarsBySrcs(Seq#Singleton(Seq#Index(obj#4,i))), alloc)
+			)
+		);
+  invariant (forall<alpha> $o : ref, $f: Field alpha ::
+	($o == null || read($tarHeap, $o, $f) == read(old($tarHeap), $o, $f) || (dtype($o) == REL$RELSchema && dtype(Seq#Index(getTarsBySrcs_inverse($o), 0)) == ER$ERSchema && $f==alloc)));
+  free invariant $HeapSucc(old($tarHeap), $tarHeap);
+  free invariant $HeapSucc(old($linkHeap), $linkHeap);
+{ 
+	
+	stk := Seq#Build(stk, $Box(Seq#Index(obj#4, $i)));
+	call stk, s := OpCode#Store(stk);
+	
+	// placed just after the condition check.
+
+	
+	call stk := OpCode#GetASM(stk);
+	
+	assert Seq#Length(stk) >= 1;
+	assert $Unbox(Seq#Index(stk, Seq#Length(stk)-1)) != null;
+	stk := Seq#Build(Seq#Take(stk, Seq#Length(stk)-1), $Box($linkHeap[$Unbox(Seq#Index(stk, Seq#Length(stk)-1)), FieldOfDecl(dtype($Unbox(Seq#Index(stk, Seq#Length(stk)-1))), _Field$links): Field (Set ref)]));
+
+	
+	
+	
+	
+	call stk := OpCode#Push(stk, _TransientLink);
+	call stk := OpCode#Push(stk, _#native);
+
+	assert Seq#Length(stk) >= 2;
+	havoc obj#11;
+    assume obj#11 != null && !read($linkHeap, obj#11, alloc) && dtype(obj#11) == 
+	classifierTable[($Unbox(Seq#Index(stk, Seq#Length(stk)-1)): String), 
+					($Unbox(Seq#Index(stk, Seq#Length(stk)-2)): String)];
+	$linkHeap := update($linkHeap, obj#11, alloc, true);
+	assume $IsGoodHeap($linkHeap);
+	assume $HeapSucc(old($linkHeap), $linkHeap);
+	stk := Seq#Build(Seq#Take(stk, Seq#Length(stk)-2), $Box(obj#11));
+
+	call stk := OpCode#Dup(stk);
+	call stk := OpCode#Push(stk, _S2S);
+	
+	call stk := NTransientLink#setRule
+	(stk, 
+	 $Unbox(Seq#Index(stk, Seq#Length(stk)-2)),
+	 $Unbox(Seq#Index(stk, Seq#Length(stk)-1)));
+
+	call stk := OpCode#Dup(stk);
+	call stk := OpCode#Push(stk, _s);
+	call stk := OpCode#Load(stk, s);
+	
+	call stk := NTransientLink#addSourceElement
+	(stk, 
+	 $Unbox(Seq#Index(stk, Seq#Length(stk)-3)),
+	 $Unbox(Seq#Index(stk, Seq#Length(stk)-2)),
+	 $Unbox(Seq#Index(stk, Seq#Length(stk)-1)));
+
+	call stk := OpCode#Dup(stk);
+	call stk := OpCode#Push(stk, _t);
+	call stk := OpCode#Push(stk, _RELSchema);
+	call stk := OpCode#Push(stk, _REL);
+	
+	assert Seq#Length(stk) >= 2;
+	havoc obj#23;
+    assume obj#23 != null && !read($tarHeap, obj#23, alloc) && dtype(obj#23) == 
+	classifierTable[($Unbox(Seq#Index(stk, Seq#Length(stk)-1)): String), 
+					($Unbox(Seq#Index(stk, Seq#Length(stk)-2)): String)];
+	$tarHeap := update($tarHeap, obj#23, alloc, true);
+	assume $IsGoodHeap($tarHeap);
+	assume $HeapSucc(old($tarHeap), $tarHeap);
+	assume getTarsBySrcs(Seq#Singleton(s)) == obj#23;
+	stk := Seq#Build(Seq#Take(stk, Seq#Length(stk)-2), $Box(obj#23));
+	
+	
+	
+	
+	call stk := NTransientLink#addTargetElement
+	(stk, 
+	 $Unbox(Seq#Index(stk, Seq#Length(stk)-3)),
+	 $Unbox(Seq#Index(stk, Seq#Length(stk)-2)),
+	 $Unbox(Seq#Index(stk, Seq#Length(stk)-1)));
+	
+	assert $linkHeap[obj#11, TransientLink#rule] == _S2S;
+	assert Map#Elements($linkHeap[obj#11, TransientLink#target])[_t] == obj#23;
+	assert Map#Elements($linkHeap[obj#11, TransientLink#source])[_s] == s;
+	
+	
+	call stk := OpCode#Pusht(stk);
+	stk := Seq#Take(stk, Seq#Length(stk)-3);
+	$i := $i+1;
+	
+	assert $HeapSucc(old($tarHeap), $tarHeap);
+	assert $HeapSucc(old($linkHeap), $linkHeap);
+
+
+	
+}
+}
+
+
+
